src/goose_lang/lib/encoding/encoding.v
@@ -288,6 +288,41 @@ Proof.
   lia.
 Qed.
 
+(* For when you use UInt64Put not at the beginning of a subslice, and already
+   got your [is_slice_small] written with a [++]. *)
+Theorem wp_UInt64Put_skip {stk E} s n x (pre vs : list val) :
+  length pre = int.nat n →
+  length vs >= u64_bytes →
+  {{{ is_slice_small s byteT 1%Qp (pre ++ vs) }}}
+    UInt64Put (slice_val $ slice_skip s byteT n) #x @ stk; E
+  {{{ RET #(); is_slice_small s byteT 1%Qp (pre ++ u64_le_bytes x ++ (drop u64_bytes vs)) }}}.
+Proof.
+  iIntros (Hpre Hlen Φ) "Hsl HΦ".
+  wp_lam.
+  wp_let.
+  wp_lam.
+  wp_pures.
+  rewrite /is_slice_small. iDestruct "Hsl" as "(Hptr&[%Hsz %Hwf])".
+  rewrite array_app.
+  rewrite app_length in Hsz.
+  iDestruct "Hptr" as "[Hhead Hptr]".
+  iDestruct (array_split 8 with "Hptr") as "[Henc Hrest]"; first lia.
+  { word. }
+  wp_apply (wp_EncodeUInt64 with "[Henc]").
+  { iSplit.
+    - iNext. iExactEq "Henc". repeat f_equal. word.
+    - iPureIntro. rewrite take_length; word. }
+  iIntros "Henc".
+  change (Z.to_nat 8) with 8%nat.
+  iApply "HΦ". iSplit.
+  - rewrite !array_app. iFrame "Hhead Hrest".
+    iExactEq "Henc". repeat f_equal. word.
+  - iPureIntro.
+    rewrite !app_length drop_length u64_le_bytes_length.
+    word.
+Qed.
+
+
 Definition u32_le_bytes (x: u32) : list val :=
   b2val <$> u32_le x.
 
